commit

src/mink/main.lean
@@ -1,102 +1,77 @@
 import tactic
 import tactic.induction
-import logic.function.iterate
 
-inductive Expr
-| K : Expr
-| S : Expr
-| M : Expr
-| App : Expr → Expr → Expr
-open Expr
+noncomputable theory
+open_locale classical
 
-infixl ` ~ `:100 := App
+namespace test
 
-@[simp]
-def reduce : Expr → Expr
-| (K ~ a ~ b) := a
-| (S ~ a ~ b ~ c) := a ~ c ~ (b ~ c)
-| (M ~ K) := K
-| (M ~ S) := S
-| (M ~ a) := M ~ reduce a
-| (a ~ b) := reduce a ~ b
-| a := a
+inductive T
+| nil : T
+| pair : T → T → T
+open T
 
-@[simp]
-def reduces (a b : Expr) :=
-∃ (n : ℕ), (reduce^[n] a) = b
+@[reducible] def zero : T := nil
+@[reducible] instance : has_zero T := ⟨nil⟩
 
-infix ` ==> `:50 := reduces
+@[reducible] def one : T := pair 0 0
+@[reducible] instance : has_one T := ⟨one⟩
 
-def T (a : Expr) :=
-reduces a K
+def is_nil : T → Prop
+| nil := true
+| (pair _ _) := false
+
+def is_pair : T → Prop
+| nil := false
+| (pair _ _) := true
+
+instance : has_coe_to_sort T Prop := ⟨is_pair⟩
 
 -----
 
-@[simp]
-lemma not_T {a : Expr} : ¬T a ↔ ∀ (n : ℕ), ¬(reduce^[n]) a = K :=
-by simp [T]
+def True : T := 1
+def False : T := 0
 
-lemma reduce_succ {a : Expr} {n : ℕ} :
-  (reduce^[n.succ]) a = (reduce^[n]) (reduce a) :=
-by apply function.iterate_succ_apply
+def Pro : T → T
+| 0 := True
+| 1 := True
+| _ := False
 
-lemma reduce_succ' {a : Expr} {n : ℕ} :
-  (reduce^[n.succ]) a = reduce (reduce^[n] a) :=
-by apply function.iterate_succ_apply'
+def not : T → T
+| nil := 1
+| (pair _ _) := 0
 
-lemma T_K : T K :=
-by { use 0, refl }
+def and : T → T → T
+| 0 _ := 0
+| _ a := 1
 
-lemma not_T_of_reduce_id {a : Expr}
-  (h₁ : a ≠ K) (h₂ : reduce a = a) : ¬T a := by
-{ simp, intro n, induction n,
-  { simpa },
-  { simpa [h₂] }}
+def or : T → T → T
+| 0 a := a
+| _ _ := 1
 
-lemma not_T_S : ¬T S :=
-by simp [not_T_of_reduce_id]
-
-lemma not_T_M : ¬T M :=
-by simp [not_T_of_reduce_id]
+def iff : T → T → T
+| 0 0 := True
+| 1 1 := True
+| _ _ := False
 
 -----
 
-@[reducible]
-def I := S ~ K ~ K
-
-@[simp]
-lemma T_I_app_iff {a : Expr} : T (I ~ a) ↔ T a := by
-{ split; rintro ⟨n, h⟩,
-  { cases n, { cases h },
-    cases n, { cases h },
-    simp at h, use [n, h] },
-  { use n + 2, simpa }}
-
-lemma T_M_app_iff {a : Expr} : T (M ~ a) ↔ T a := by
-{ split; rintro ⟨n, h⟩, cases n, { cases h }, use n, swap, use n + 1,
-  repeat {
-    induction' n with n ih; simp at *,
-    { cases a; simp * at * },
-    { cases a; simp at *; try { assumption },
-      { contrapose! h, clear h ih, revert n,
-        simp [←not_T, not_T_of_reduce_id] },
-      { exact ih h }}}}
-
-lemma not_T_of_reduce_app {a : Expr}
-  (h : ∀ (n : ℕ), ∃ (b c : Expr), (reduce^[n]) a = b ~ c) : ¬T a :=
-by { rw not_T, intro n, specialize h n, rcases h with ⟨b, c, h⟩, simp [h] }
-
-lemma T_iff_T_reduces {a b : Expr} (h : a ==> b) : T a ↔ T b := by
+lemma not_not {a : T} (h : Pro a) : iff (not (not a)) a := by
 {
-  sorry
+  replace h : a = 0 ∨ a = 1,
+  {
+    cases a with a b,
+    { left, refl },
+    {
+      right,
+      cases a, swap, { exact h.elim },
+      cases b, swap, { exact h.elim },
+      triv,
+    },
+  },
+  rcases h with rfl | rfl; triv,
 }
 
-#exit
+-----
 
-lemma not_T_SII_SII : ¬T (S ~ I ~ I ~ (S ~ I ~ I)) := by {
-  apply not_T_of_reduce_app, intro n,
-  induction n using nat.strong_induction_on with n ih, dsimp at ih,
-  cases n; simp,
-  cases n; simp,
-  cases n; simp,
-}
+end test
