src/mink/old/main.lean
@@ -1,0 +1,102 @@
+import tactic
+import tactic.induction
+import logic.function.iterate
+
+inductive Expr
+| K : Expr
+| S : Expr
+| M : Expr
+| App : Expr → Expr → Expr
+open Expr
+
+infixl ` ~ `:100 := App
+
+@[simp]
+def reduce : Expr → Expr
+| (K ~ a ~ b) := a
+| (S ~ a ~ b ~ c) := a ~ c ~ (b ~ c)
+| (M ~ K) := K
+| (M ~ S) := S
+| (M ~ a) := M ~ reduce a
+| (a ~ b) := reduce a ~ b
+| a := a
+
+@[simp]
+def reduces (a b : Expr) :=
+∃ (n : ℕ), (reduce^[n] a) = b
+
+infix ` ==> `:50 := reduces
+
+def T (a : Expr) :=
+reduces a K
+
+-----
+
+@[simp]
+lemma not_T {a : Expr} : ¬T a ↔ ∀ (n : ℕ), ¬(reduce^[n]) a = K :=
+by simp [T]
+
+lemma reduce_succ {a : Expr} {n : ℕ} :
+  (reduce^[n.succ]) a = (reduce^[n]) (reduce a) :=
+by apply function.iterate_succ_apply
+
+lemma reduce_succ' {a : Expr} {n : ℕ} :
+  (reduce^[n.succ]) a = reduce (reduce^[n] a) :=
+by apply function.iterate_succ_apply'
+
+lemma T_K : T K :=
+by { use 0, refl }
+
+lemma not_T_of_reduce_id {a : Expr}
+  (h₁ : a ≠ K) (h₂ : reduce a = a) : ¬T a := by
+{ simp, intro n, induction n,
+  { simpa },
+  { simpa [h₂] }}
+
+lemma not_T_S : ¬T S :=
+by simp [not_T_of_reduce_id]
+
+lemma not_T_M : ¬T M :=
+by simp [not_T_of_reduce_id]
+
+-----
+
+@[reducible]
+def I := S ~ K ~ K
+
+@[simp]
+lemma T_I_app_iff {a : Expr} : T (I ~ a) ↔ T a := by
+{ split; rintro ⟨n, h⟩,
+  { cases n, { cases h },
+    cases n, { cases h },
+    simp at h, use [n, h] },
+  { use n + 2, simpa }}
+
+lemma T_M_app_iff {a : Expr} : T (M ~ a) ↔ T a := by
+{ split; rintro ⟨n, h⟩, cases n, { cases h }, use n, swap, use n + 1,
+  repeat {
+    induction' n with n ih; simp at *,
+    { cases a; simp * at * },
+    { cases a; simp at *; try { assumption },
+      { contrapose! h, clear h ih, revert n,
+        simp [←not_T, not_T_of_reduce_id] },
+      { exact ih h }}}}
+
+lemma not_T_of_reduce_app {a : Expr}
+  (h : ∀ (n : ℕ), ∃ (b c : Expr), (reduce^[n]) a = b ~ c) : ¬T a :=
+by { rw not_T, intro n, specialize h n, rcases h with ⟨b, c, h⟩, simp [h] }
+
+lemma T_iff_T_reduces {a b : Expr} (h : a ==> b) : T a ↔ T b := by
+{
+  sorry
+}
+
+#exit
+
+lemma not_T_SII_SII : ¬T (S ~ I ~ I ~ (S ~ I ~ I)) := by {
+  apply not_T_of_reduce_app, intro n,
+  induction n using nat.strong_induction_on with n ih, dsimp at ih,
+  cases n; simp,
+  cases n; simp,
+  cases n; simp,
+}
